BrokerRegistry.v
@@ -1,0 +1,149 @@
+Require Import
+        Coq.FSets.FMapWeakList.
+Require Import
+        Events
+        LibModel
+        Maps
+        Messages
+        States
+        Types.
+
+
+Section Aux.
+
+  Definition get_brokersMap (wst: WorldState) : BrokersMap.t :=
+    broker_registry_brokersMap (wst_broker_registry_state wst).
+
+  Definition get_broker_info
+             (m: BrokersMap.t) (owner broker: address)
+    : option Broker :=
+    match BrokersMap.find m owner with
+    | None => None
+    | Some brokers =>
+      match Brokers.find brokers broker with
+      | None => None
+      | Some broker_info => Some broker_info
+      end
+    end.
+
+  Definition upd_broker_info
+             (m: BrokersMap.t) (owner broker: address) (broker_info: Broker)
+    : BrokersMap.t :=
+    BrokersMap.upd m
+                   owner
+                   (Brokers.upd (BrokersMap.get m owner)
+                                broker
+                                broker_info).
+
+  Definition del_broker_info
+             (m: BrokersMap.t) (owner broker: address)
+    : BrokersMap.t :=
+    BrokersMap.upd m
+                   owner
+                   (Brokers.del (BrokersMap.get m owner) broker).
+
+End Aux.
+
+
+Section Func_getBroker.
+
+  Definition func_getBroker
+             (wst0 wst: WorldState) (sender owner broker: address)
+  : (WorldState * Result) :=
+    let brokersMap := get_brokersMap wst in
+    match get_broker_info brokersMap owner broker with
+    | None => (wst,
+              {| res_events := nil;
+                 res_return := Some (Return (false, 0))|})
+    | Some broker_info => (wst,
+                          {| res_events := nil;
+                             res_return := Some (Return (true, broker_interceptor broker_info)) |})
+    end.
+
+End Func_getBroker.
+
+
+Section Func_registerBroker.
+
+  Definition func_registerBroker
+             (wst0 wst: WorldState) (sender broker interceptor: address)
+  : (WorldState * Result) :=
+    match broker with
+    | O => (wst0, make_revert_result)
+    | _ =>
+      let brokersMap := get_brokersMap wst in
+      match get_broker_info brokersMap sender broker with
+      | Some _ => (wst0, make_revert_result)
+      | None =>
+        let brokerInfo := {| broker_owner := sender;
+                             broker_addr := broker;
+                             broker_interceptor := interceptor;
+                          |}
+        in
+        let brokersMap' := upd_broker_info brokersMap sender broker brokerInfo in
+        (wst_update_broker_registry wst {| broker_registry_brokersMap := brokersMap' |},
+         {|
+           res_events := EvtBrokerRegistered sender broker interceptor :: nil;
+           res_return := None;
+         |})
+      end
+    end.
+
+End Func_registerBroker.
+
+
+Section Func_unregisterBroker.
+
+  Definition func_unregisterBroker
+             (wst0 wst: WorldState) (sender broker: address)
+  : WorldState * Result :=
+    match broker with
+    | O => (wst0, make_revert_result)
+    | _ =>
+      let brokersMap := get_brokersMap wst in
+      match get_broker_info brokersMap sender broker with
+      | None => (wst0, make_revert_result)
+      | Some broker_info =>
+        let brokersMap' := del_broker_info brokersMap sender broker in
+        (wst_update_broker_registry wst {| broker_registry_brokersMap := brokersMap' |},
+         {|
+           res_events := EvtBrokerUnregistered sender broker (broker_interceptor broker_info) :: nil;
+           res_return := None;
+         |})
+      end
+    end.
+
+End Func_unregisterBroker.
+
+
+Section Func_unregsterAllBrokers.
+
+  Definition func_unregisterAllBrokers
+             (wst0 wst: WorldState) (sender: address)
+  : WorldState * Result :=
+    let brokersMap := get_brokersMap wst in
+    let brokersMap' := BrokersMap.del brokersMap sender in
+    (wst_update_broker_registry wst {| broker_registry_brokersMap := brokersMap' |},
+     {|
+       res_events := EvtAllBrokersUnregistered sender :: nil;
+       res_return := None;
+     |}).
+
+End Func_unregsterAllBrokers.
+
+
+Definition BrokerRegistry_step
+           (wst0 wst: WorldState) (msg: BrokerRegistryMsg)
+  : (WorldState * Result) :=
+  match msg with
+  | msg_getBroker sender owner broker =>
+    func_getBroker wst0 wst sender owner broker
+  (* | msg_getBrokers sender owner s e => *)
+  (*   func_getBrokers wst0 wst sender owner s e *)
+  | msg_registerBroker sender broker interceptor =>
+    func_registerBroker wst0 wst sender broker interceptor
+  | msg_unregisterBroker sender broker =>
+    func_unregisterBroker wst0 wst sender broker
+  | msg_unregisterAllBrokers sender =>
+    func_unregisterAllBrokers wst0 wst sender
+  end.
